src/dafny/util/int.dfy
@@ -12,6 +12,15 @@
  * under the License.
  */
 module Int {
+  // Powers of Two
+  const TWO_8   : int := 0x1_00;
+  const TWO_16  : int := 0x1_0000;
+  const TWO_32  : int := 0x1_0000_0000;
+  const TWO_64  : int := 0x1_0000_0000_0000_0000;
+  const TWO_128 : int := 0x1_0000_0000_0000_0000_0000_0000_0000_0000;
+  const TWO_160 : int := 0x1_0000_0000_0000_0000_0000_0000_0000_0000_0000_0000;
+  const TWO_256 : int := 0x1_0000_0000_0000_0000_0000_0000_0000_0000_0000_0000_0000_0000_0000_0000_0000_0000;
+
   // Signed Integers
   const MIN_I8  : int := -0x80;
   const MAX_I8  : int :=  0x80 - 1;
@@ -28,13 +37,13 @@ module Int {
   newtype{:nativeType "long"}  i64 = i:int  | MIN_I64 <= i <= MAX_I64
 
   // Unsigned Integers
-  const MAX_U8 : int :=  0x1_00 - 1;
-  const MAX_U16 : int := 0x1_0000 - 1;
-  const MAX_U32 : int := 0x1_0000_0000 - 1;
-  const MAX_U64 : int := 0x10000000000000000 - 1;
-  const MAX_UINT128 : int :=  0x1_0000_0000_0000_0000_0000_0000_0000_0000 - 1;
-  const MAX_UINT160: int := 0x1_0000_0000_0000_0000_0000_0000_0000_0000_0000_0000 - 1;
-  const MAX_UINT256: int := 0x1_0000_0000_0000_0000_0000_0000_0000_0000_0000_0000_0000_0000_0000_0000_0000_0000 - 1
+  const MAX_U8 : int :=  TWO_8 - 1;
+  const MAX_U16 : int := TWO_16 - 1;
+  const MAX_U32 : int := TWO_32 - 1;
+  const MAX_U64 : int := TWO_64 - 1;
+  const MAX_UINT128 : int := TWO_128 - 1;
+  const MAX_UINT160: int := TWO_160 - 1;
+  const MAX_UINT256: int := TWO_256 - 1
 
   newtype{:nativeType "byte"} u8 = i:int    | 0 <= i <= MAX_U8
   newtype{:nativeType "ushort"} u16 = i:int | 0 <= i <= MAX_U16
@@ -43,4 +52,34 @@ module Int {
   newtype u128 = i:int | 0 <= i <= MAX_UINT128
   newtype u160 = i:int | 0 <= i <= MAX_UINT160
   newtype u256 = i:int | 0 <= i <= MAX_UINT256
+
+  // =========================================================
+  // Conversion to/from byte sequences
+  // =========================================================
+
+  function read_u8(bytes: seq<u8>, address:nat) : u8
+  requires address < |bytes| {
+    bytes[address]
+  }
+
+  function read_u16(bytes: seq<u8>, address:nat) : u16
+  requires (address+1) < |bytes| {
+    var b1 := bytes[address] as u16;
+    var b2 := bytes[address+1] as u16;
+    (b1 * (TWO_8 as u16)) + b2
+  }
+
+  function read_u32(bytes: seq<u8>, address:nat) : u32
+  requires (address+3) < |bytes| {
+    var b1 := read_u16(bytes, address) as u32;
+    var b2 := read_u16(bytes, address+2) as u32;
+    (b1 * (TWO_16 as u32)) + b2
+  }
+
+  function read_u64(bytes: seq<u8>, address:nat) : u64
+  requires (address+7) < |bytes| {
+    var b1 := read_u32(bytes, address) as u64;
+    var b2 := read_u32(bytes, address+4) as u64;
+    (b1 * (TWO_32 as u64)) + b2
+  }
 }
